\documentclass[12pt]{article}
% \documentclass[12pt]{beamer}
\usepackage{amsmath,amsfonts,amssymb,amsthm}
\usepackage{color}
\usepackage[T1]{fontenc}
\usepackage{mathtools}
\usepackage{graphicx}
\usepackage{subcaption}
\usepackage{kotex}
\usepackage{bm}
\usepackage[shortlabels]{enumitem}
\usepackage{tcolorbox}
\usepackage{mathrsfs}
\usepackage{newtxtext}
\usepackage[lite,nofontinfo,zswash,straightbraces]{mtpro2}
\usepackage{setspace} %줄간격 package
%-------------------------------------------------------------------------------------
% Page layout
\addtolength{\textwidth}{1.2in}
\addtolength{\oddsidemargin}{-0.6in}
\addtolength{\textheight}{2.0in}
\addtolength{\topmargin}{-1.0in}
\renewcommand \baselinestretch{1.2}
\parskip = 6pt
% New command
\newcommand {\AND}{\quad\mbox{and}\quad}
\newcommand {\for}{\quad\mbox{ for }}
\newcommand {\half}{{\tfrac 12}}
% \newcommand {\bm} [1] {\mbox{\boldmath{$#1$}}}
\newcommand{\bs}{\boldsymbol}
\DeclareMathOperator{\Tr}{Tr}
\DeclareMathOperator{\Cov}{Cov}
\DeclareMathOperator{\Var}{Var}
\DeclareMathOperator{\E}{\mathbf{E}}
\DeclareMathOperator{\vvv}{vec}
\DeclareMathOperator{\vvvh}{vech}
% \setmainfont{TEX Gyre Termes}
% \setmathfont[bold-style=TeX]{TG Termes Math}
\begin{document}
\setstretch{1.4} %줄간격 조정
\title{Stochastic Variational Inference for SSGP}
%------------------------------------------------------------------------------------%
%------------------------------------------------------------------------------------%
% \setcounter{section}{1}

\section{Stochastic Variational Inference in Gaussian Regression}
  For the sprectral decomposition of the Gaussian process, we use the following expansion:
  \begin{equation}
    f(x) \approx \sum_{r=1}^{m}\left[a_{r}\cos\left\{\left(s_{r}\odot x\right)'\lambda\right\}+b_{r}\sin\left\{\left(s_{r}\odot x\right)'\lambda\right\}\right]
  \end{equation}
  where $\lambda=(\lambda_{1},\ldots,\lambda_{d})'$ ad $\odot$ denots the Hadamard product.
  \begin{itemize}
    \item $\alpha=(a_{1},\ldots,a_{m},b_{1},\ldots,b_{m})'$
    \item $y = (y_{1},\ldots,y_{n})'$
    \item $Z = (Z_{1},\ldots,Z_{n})'$
    \item $Z_{i} = (\cos((s_{1}\odot x_{i})'\lambda),\ldots, \cos((s_{m}\odot x_{i})'\lambda),\sin((s_{1}\odot x_{i})'\lambda),\ldots,\sin((s_{m}\odot x_{i})'\lambda)$
    \item $\epsilon = (\epsilon_{1},\ldots,\epsilon_{n})'$
  \end{itemize}
  Then,
  \begin{equation}
    y = Z\alpha+\epsilon, \quad \epsilon\sim\mathcal{N}\left(0,\gamma^{2}I_{n}\right)
  \end{equation}
  with the following priors
  \begin{itemize}
    \item $\alpha\sim\mathcal{N}\left(0,\dfrac{\sigma^{2}}{m}I_{2m}\right)$
    \item $\lambda \sim \mathcal{N}\left(\mu_{\lambda}^{0},\Sigma_{\lambda}^{0}\right)$
    \item $\sigma \sim \mathrm{HF}\left(A_{\sigma}\right)$
    \item $\gamma \sim \mathrm{HF}\left(A_{\gamma}\right)$
  \end{itemize}
  where the density of half-Cauchy distribution is as follows:
\begin{equation}
  \pi(\sigma) = \dfrac{2A_{\sigma}}{\pi\left(A_{\sigma}^{2}+\sigma^{2}\right)}.
\end{equation}
  The fixed variational posteriors are
  \begin{itemize}
    \item $q(\alpha)=\mathcal{N}\left(\mu_{\alpha}^{q},\Sigma_{\alpha}^{q}\right)$
    \item $q(\lambda)=\mathcal{N}\left(\mu_{\lambda}^{q},\Sigma_{\lambda}^{q}\right)$
    \item $q(\sigma) = b_{\sigma}^{a_{\sigma}}/\Gamma\left(a_{\sigma}\right) \left(\sigma^{2}\right)^{-(a_{\sigma}+1)}e^{-b_{\sigma}/\sigma}$
    \item $q(\gamma) = b_{\gamma}^{a_{\gamma}}/\Gamma\left(a_{\gamma}\right) \left(\gamma^{2}\right)^{-(a_{\gamma}+1)}e^{-b_{\gamma}/\gamma}$
  \end{itemize}
\subsection{Lower bound}
Let $h(\theta) = p(y\,|\,\theta)\pi(\theta)$ where $\theta = (\alpha,\lambda,\sigma,\gamma)$.
\begin{align}
  \log h(\theta) &= -\dfrac{n}{2}\log \gamma^{2}-\dfrac{1}{2\gamma^{2}}\left(y-Z\alpha\right)'\left(y-Z\alpha\right)\\
  &\quad -m\log\dfrac{\sigma^{2}}{m}-\dfrac{m}{2\sigma^{2}}\alpha'\alpha\\
  &\quad +\log(2A_{\sigma})-\log\left(\pi\left(A_{\sigma}^{2}+\sigma^{2}\right)\right)+\log\left(2A_{\gamma}\right)-\log\left(\pi\left(A_{\gamma}^{2}+\gamma^{2}\right)\right)\\
  &\quad +\dfrac{1}{2}\log\left|{\Sigma_{\lambda}^{0}}^{-1}\right|-\dfrac{1}{2}\left(\lambda-\mu_{\lambda}^{0}\right)'{\Sigma_{\lambda}^{0}}^{-1}\left(\lambda-\mu_{\lambda}^{0}\right)
\end{align}
The variational posterior is denoted by $q_{\lambda}(\theta)$.
\begin{align}
  \log q_{\lambda}(\theta) &= -m\log\left|\Sigma_{\alpha}^{q}\right|-\dfrac{1}{2}\left(\alpha-\mu_{\alpha}^{q}\right)'{\Sigma_{\alpha}^{q}}^{-1}\left(\alpha-\mu_{\alpha}^{q}\right)\\
  &\quad -\dfrac{d}{2}\log\left|\Sigma_{\lambda}^{q}\right|-\dfrac{1}{2}\left(\lambda-\mu_{\lambda}^{q}\right)'{\Sigma_{\lambda}^{q}}^{-1}\left(\lambda-\mu_{\lambda}^{q}\right)\\
  &\quad +a_{\sigma}\log b_{\sigma}-\log\Gamma\left(a_{\sigma}\right)-\left(a_{\sigma}+1\right)\log \sigma^{2}-\dfrac{b_{\sigma}}{\sigma^{2}}\\
  &\quad +a_{\gamma}\log b_{\gamma}-\log\Gamma\left(a_{\gamma}\right)-\left(a_{\gamma}+1\right)\log \gamma^{2}-\dfrac{b_{\gamma}}{\gamma^{2}}
\end{align}
\end{document}